pending/default.lean
@@ -3,12 +3,17 @@
 import data.stream data.lazy_list
 
 -- To be merged into data.stream
-def stream.corec' {α β} (f : α → β × α) (a : α) : stream β :=
-stream.corec (prod.fst ∘ f) (prod.snd ∘ f) a
+namespace stream
+def corec' {α β} (f : α → β × α) (a : α) : stream β :=
+corec (prod.fst ∘ f) (prod.snd ∘ f) a
 
-def stream.corec'_eq {α β} (f : α → β × α) (a : α) :
-  stream.corec' f a = (f a).1 :: stream.corec' f (f a).2 :=
-stream.corec_eq _ _ _
+def corec'_eq {α β} (f : α → β × α) (a : α) :
+  corec' f a = (f a).1 :: corec' f (f a).2 :=
+corec_eq _ _ _
+
+lemma map_tail {α β} (f : α → β) (s : stream α) : map f (tail s) = tail (map f s) :=
+rfl
+end stream
 
 -- To be merged into data.lazy_list
 def lazy_list.to_list {α} : lazy_list α → list α
@@ -22,4 +27,11 @@ def list.filter_map {α β} (f : α → option β) : list α → list β
   match f a with 
   | none   := list.filter_map l 
   | some b := b :: list.filter_map l 
-  end 
+  end
+
+-- To be merged into init.data.option.instances
+def option_map {α β} (f : α → β) (o : option α) : option β :=
+option_bind o (some ∘ f)
+
+@[simp] theorem option.map_id {α} : (option_map id : option α → option α) = id :=
+funext (λo, by cases o; refl)
